improve shallow embedding array reasoning support

isa/Gencot_CArray_Lemmas.thy
@@ -7,10 +7,13 @@ text \<open>Lift arrays to the wrapper records.
       It consists of the following functions.
       Array accesses are always guarded by function vld.\<close>
 consts 
+  arr :: "'el list \<Rightarrow> 'arr"
   siz :: "'arr \<Rightarrow> nat"
   vld :: "'arr \<Rightarrow> nat \<Rightarrow> bool"
   elm :: "'arr \<Rightarrow> nat \<Rightarrow> 'el"
-  upd :: "'arr \<Rightarrow> nat \<Rightarrow> 'el \<Rightarrow> 'arr"
+  elm_update :: "nat \<Rightarrow> ('el \<Rightarrow> 'el) \<Rightarrow> 'arr \<Rightarrow> 'arr"
+  elm_modified :: "nat \<Rightarrow> ('el \<Rightarrow> 'el \<Rightarrow> bool) \<Rightarrow> 'arr \<Rightarrow> 'arr \<Rightarrow> bool"
+  arr_fill :: "(nat \<Rightarrow> 'el) \<Rightarrow> 'arr"
 
 text \<open>For every actual wrapper record the following locale will be interpreted.
       It extends CArrFuns by the laws of the abstract data type, 
@@ -22,7 +25,7 @@ locale CArrLems = CArrFuns fld wrp
     wrp :: "('n, 'el) FixedList \<Rightarrow> 'arr" +
   assumes 
     fld_inverse: "\<And>x. wrp (fld x) = x" and 
-    wrp_inverse: "\<And>x. fld (wrp x) = x" 
+    wrp_inverse: "\<And>x. fld (wrp x) = x"
 begin
 
 text \<open>Define conversion functions between lists and the wrapper record.\<close>
@@ -34,12 +37,17 @@ definition arrFxd :: "'el list \<Rightarrow> 'arr"
 text \<open>Define the abstract data type functions for the wrapper record.\<close>
 definition sizFxd :: "'arr \<Rightarrow> nat"
   where "sizFxd a \<equiv> length (lstFxd a)"
-definition vldFxd :: "'arr => nat => bool"
+definition vldFxd :: "'arr \<Rightarrow> nat \<Rightarrow> bool"
   where "vldFxd a i \<equiv> i < sizFxd a"
 definition elmFxd :: "'arr \<Rightarrow> nat \<Rightarrow> 'el"
   where "elmFxd a i \<equiv> nth (lstFxd a) i"
-definition updFxd :: "'arr \<Rightarrow> nat \<Rightarrow> 'el \<Rightarrow> 'arr"
-  where "updFxd a i e \<equiv> arrFxd (list_update (lstFxd a) i e)"
+definition elm_updateFxd :: "nat \<Rightarrow> ('el \<Rightarrow> 'el) \<Rightarrow> 'arr \<Rightarrow> 'arr"
+  where "elm_updateFxd i f a \<equiv> arrFxd (list_update (lstFxd a) i (f (elmFxd a i)))"
+definition elm_modifiedFxd :: "nat \<Rightarrow> ('el \<Rightarrow> 'el \<Rightarrow> bool) \<Rightarrow> 'arr \<Rightarrow> 'arr \<Rightarrow> bool"
+  where elm_modified_def: "elm_modifiedFxd i m a1 a2 \<equiv> 
+    m (elmFxd a1 i) (elmFxd a2 i) \<and> (\<forall>j \<noteq> i. vldFxd a1 j \<longrightarrow> elmFxd a1 j = elmFxd a2 j)"
+definition arr_fillFxd :: "(nat \<Rightarrow> 'el) \<Rightarrow> 'arr"
+  where "arr_fillFxd f \<equiv> arrFxd [f x . x \<leftarrow> [0 ..< LENGTH('n)]]"
 
 text \<open>Arrays are never empty.\<close>
 lemma arrNotNil: "\<forall>x::'arr .  lstFxd x \<noteq> []"
@@ -54,18 +62,33 @@ lemma sizArr: "sizFxd a = LENGTH('n)"
   by (simp add: length_FixedList)
 lemma vldArr: "vldFxd a n = (n < LENGTH('n))"
   by (simp add: vldFxd_def sizArr)
-lemma updArr: "vldFxd a i \<Longrightarrow> elmFxd (updFxd a i e) i = e"
-  apply(auto simp add: updFxd_def elmFxd_def lstFxd_def arrFxd_def wrp_inverse vldArr)
-  apply(subst Abs_FixedList_inverse)
-  apply(cut_tac x = "(fld a)" in Rep_FixedList )
+lemma elmUpdElm: "elm_updateFxd i (f \<circ> (\<lambda>_. g (elmFxd a i))) a = elm_updateFxd i (f \<circ> g) a"
+  by (simp add: elm_updateFxd_def)
+lemma elmUpdDistrib: "(i < LENGTH('n)) \<Longrightarrow> elm_updateFxd i (f \<circ> g) = (elm_updateFxd i f) \<circ> (elm_updateFxd i g)"
+  for f:: "'el \<Rightarrow> 'el"
+  apply (unfold elm_updateFxd_def elmFxd_def arrFxd_def lstFxd_def)
+  apply(rule ext)
   apply(auto)
   apply(cut_tac x = "(fld a)" in Rep_FixedList )
-  by auto
-lemma updArrFrame: "vldFxd a i \<and> vldFxd a j \<and> i \<noteq> j \<Longrightarrow> elmFxd (updFxd a i e) j = elmFxd a j"
-  apply(auto simp add: updFxd_def elmFxd_def lstFxd_def arrFxd_def wrp_inverse vldArr)
-  apply(subst Abs_FixedList_inverse)
+  apply(subst wrp_inverse)+
+  apply(subst Abs_FixedList_inverse,simp)+
+  by(auto)
+lemma elmElmUpd: "vldFxd a i \<Longrightarrow> elmFxd (elm_updateFxd i f a) i = f (elmFxd a i)"
+  apply(auto simp add: elm_updateFxd_def elmFxd_def arrFxd_def lstFxd_def vldArr)
   apply(cut_tac x = "(fld a)" in Rep_FixedList )
+  apply(subst wrp_inverse)
+  apply(subst Abs_FixedList_inverse)
   by (auto)
+lemma elmElmUpdFrame: "vldFxd a i \<and> vldFxd a j \<and> i \<noteq> j \<Longrightarrow> elmFxd (elm_updateFxd i f a) j = elmFxd a j"
+  apply(auto simp add: elm_updateFxd_def elmFxd_def arrFxd_def lstFxd_def vldArr)
+  apply(cut_tac x = "(fld a)" in Rep_FixedList )
+  apply(subst wrp_inverse)
+  apply(subst Abs_FixedList_inverse)
+  by (auto)
+lemma elmArrFill: "i < LENGTH('n) \<Longrightarrow> elmFxd (arr_fillFxd f) i = f i"
+  apply(auto simp add: elmFxd_def arr_fillFxd_def lstFxd_def arrFxd_def wrp_inverse vldArr sizArr)
+  apply(subst Abs_FixedList_inverse)
+  by auto
 
 text \<open>Array equality by extensionality. \<close>
 lemma eqArr1: "(\<And> i. (vldFxd a1 i) \<Longrightarrow> ((elmFxd a1 i) = (elmFxd a2 i))) \<Longrightarrow> (a1 = a2)"
@@ -79,40 +102,95 @@ lemma eqArr1: "(\<And> i. (vldFxd a1 i) \<Longrightarrow> ((elmFxd a1 i) = (elmF
   apply(drule arg_cong[where f = wrp])
   apply(simp add: fld_inverse)
   done
-lemma eqArr: "(a1 = a2) = (\<forall> i. (vldFxd a1 i) \<longrightarrow> ((elmFxd a1 i) = (elmFxd a2 i)))"
+lemma eqArr: "(a1 = a2) = 
+              (\<forall> i. (vldFxd a1 i) \<longrightarrow> ((elmFxd a1 i) = (elmFxd a2 i)))"
   apply(rule iffI)
    apply(rule allI)
    apply(rule impI)
    apply(auto)
   by (rule eqArr1,auto)
 
-text \<open>Conversion laws for the array functions to the abstract data type.\<close>
-text \<open>Conversion for getArr\<close>
-lemma getArrValid: "vldFxd a (unat i) \<Longrightarrow> getArrFxd (a,i) = elmFxd a (unat i)"
+lemma eqElmUpd: "vldFxd a2 i \<Longrightarrow> (a1 = elm_updateFxd i f a2) =
+                 ((elmFxd a1 i) = f (elmFxd a2 i) \<and> (\<forall> j. j \<noteq> i \<and> (vldFxd a1 j) \<longrightarrow> (elmFxd a1 j) = (elmFxd a2 j)))"
+  apply(rule iffI)
+   apply(auto)
+    apply(subst elmElmUpd,auto)
+  apply(subst elmElmUpdFrame,auto simp add: vldArr)
+  apply(subst eqArr)
+   apply(rule allI)
+  apply(rule impI)
+  apply(case_tac "ia = i")
+  apply(simp)
+   apply(subst elmElmUpd,auto simp add: vldArr)
+  apply(subst elmElmUpdFrame,auto simp add: vldArr)
+  done
+
+lemma eqArrFill: "(a = arr_fillFxd f) = 
+                 ((\<forall> i. (vldFxd a i) \<longrightarrow> ((elmFxd a i) = f i)))"
+  apply(rule iffI)
+   apply(auto)
+   apply(rule elmArrFill)
+   apply(simp add: vldArr)
+  apply(subst eqArr)
+   apply(rule allI)
+   apply(rule impI)
+  apply(subst elmArrFill)
+  by (auto simp add: vldArr)
+
+text \<open>Semantics theorems for the Gencot array functions.\<close>
+
+definition ctrct_getArrFxd :: "'arr \<times> ('m::len) word \<Rightarrow> bool"
+  where ctrct_getArrFxd_def[simp]:
+  "ctrct_getArrFxd x \<equiv> let (a,i) = x in vldFxd a (unat i)"
+theorem sem_getArr: 
+ "ctrct_getArrFxd (a,i) \<Longrightarrow> 
+  getArrFxd (a,i) = elmFxd a (unat i)"
   by (simp add: getArrFxd_def getArr'_def vldArr elmFxd_def lstFxd_def)
-lemma getArrInvalid: "\<not> vldFxd a (unat i) \<Longrightarrow> getArrFxd (a,i) = elmFxd a 0"
+theorem errsem_getArr:
+ "\<not> ctrct_getArrFxd (a,i) \<Longrightarrow> 
+  getArrFxd (a,i) = elmFxd a 0"
   apply(simp add: getArrFxd_def getArr'_def vldArr elmFxd_def)
   apply(fold lstFxd_def)
   apply(case_tac " lstFxd a")
    apply(cut_tac arrNotNil)
   by auto
 
-text \<open>Conversion for setArr\<close>
-lemma setArrValid: "vldFxd a (unat i) \<Longrightarrow> setArrFxd (a,i,v) = (updFxd a (unat i) v, ())"
-  by (simp add: setArrFxd_def setArr'_def vldArr lstFxd_def arrFxd_def updFxd_def)
-lemma setArrInvalid: "\<not> vldFxd a (unat i) \<Longrightarrow> setArrFxd (a,i,v) = (a,())"
+definition ctrct_setArrFxd :: "'arr \<times> ('m::len) word \<times> 'el \<Rightarrow> bool"
+  where ctrct_setArrFxd_def[simp]:
+  "ctrct_setArrFxd x \<equiv> let (a,i,v) = x in vldFxd a (unat i)"
+theorem sem_setArr: 
+ "ctrct_setArrFxd (a,i,v) \<Longrightarrow> 
+  setArrFxd (a,i,v) = (elm_updateFxd (unat i) (\<lambda>_.v) a, ())"
+  by (simp add: setArrFxd_def setArr'_def vldArr lstFxd_def arrFxd_def elm_updateFxd_def)
+theorem errsem_setArr:
+ "\<not> ctrct_setArrFxd (a,i,v) \<Longrightarrow> 
+  setArrFxd (a,i,v) = (a,())"
   by (simp add: setArrFxd_def setArr'_def vldArr fld_inverse)
 
-text \<open>Conversion for modifyArr\<close>
-lemma modifyArrValid: "vldFxd a (unat i) \<Longrightarrow> modifyArrFxd (a,i,f,x) = (let (e,y) = f (elmFxd a (unat i), x) in (updFxd a (unat i) e, y))"
-  by (simp add: modifyArrFxd_def modifyArr'_def split_def Let_def vldArr lstFxd_def arrFxd_def updFxd_def elmFxd_def)
-lemma modifyArrInvalid: "\<not> (vldFxd a (unat i))  ==> modifyArrFxd (a,i,f,x) = (a, x)"
+definition ctrct_modifyArrFxd :: "'arr \<times> ('m::len) word \<times> ('el \<times> 'arg \<Rightarrow> 'el \<times> 'arg) \<times> 'arg \<Rightarrow> bool"
+  where ctrct_modifyArrFxd_def[simp]:
+  "ctrct_modifyArrFxd x \<equiv> let (a,i,f,v) = x in vldFxd a (unat i)"
+theorem sem_modifyArr:
+ "ctrct_modifyArrFxd (a,i,f,x) \<Longrightarrow> 
+  modifyArrFxd (a,i,f,x) = 
+  (let (e,y) = f (elmFxd a (unat i), x) in (elm_updateFxd (unat i) (\<lambda>_.e) a, y))"
+  by (simp add: modifyArrFxd_def modifyArr'_def split_def Let_def vldArr lstFxd_def arrFxd_def elm_updateFxd_def elmFxd_def)
+theorem errsem_modifyArr:
+ "\<not> ctrct_modifyArrFxd (a,i,f,x) ==> 
+  modifyArrFxd (a,i,f,x) = (a, x)"
   by (simp add: modifyArrFxd_def modifyArr'_def vldArr fld_inverse)
 
-text \<open>Conversion for modifyArrDfl\<close>
-lemma modifyArrDfltValid: "vldFxd a (unat i)   ==> modifyArrDfltFxd (a,i,f,x) = (let (e,y) = f (elmFxd a (unat i), x) in (updFxd a (unat i) e, y))"
-  by (simp add: modifyArrDfltFxd_def modifyArrDflt'_def split_def Let_def vldArr lstFxd_def arrFxd_def updFxd_def elmFxd_def)
-lemma modifyArrDfltInvalid: "\<not> (vldFxd a (unat i))  ==> modifyArrDfltFxd (a,i,f,x) = (a, defaultVal ())"
+definition ctrct_modifyArrDfltFxd :: "'arr \<times> ('m::len) word \<times> ('el \<times> 'arg \<Rightarrow> 'el \<times> 'out) \<times> 'arg \<Rightarrow> bool"
+  where ctrct_modifyArrDfltFxd_def[simp]:
+  "ctrct_modifyArrDfltFxd x \<equiv> let (a,i,f,v) = x in vldFxd a (unat i)"
+theorem sem_modifyArrDflt:
+ "ctrct_modifyArrDfltFxd (a,i,f,x) ==> 
+  modifyArrDfltFxd (a,i,f,x) = 
+  (let (e,y) = f (elmFxd a (unat i), x) in (elm_updateFxd (unat i) (\<lambda>_.e) a, y))"
+  by (simp add: modifyArrDfltFxd_def modifyArrDflt'_def split_def Let_def vldArr lstFxd_def arrFxd_def elm_updateFxd_def elmFxd_def)
+theorem errsem_modifyArrDflt:
+ "\<not> ctrct_modifyArrDfltFxd (a,i,f,x) ==>
+  modifyArrDfltFxd (a,i,f,x) = (a, defaultVal ())"
   by (simp add: modifyArrDfltFxd_def modifyArrDflt'_def vldArr fld_inverse)
 
 end
